Introduce reborrowing machinery

nola/iris/borrow.v
@@ -8,28 +8,43 @@ From iris.base_logic Require Import lib.invariants.
 From iris.proofmode Require Import proofmode.
 
 Implicit Type PROP : Type.
+Implicit Type (α : lft) (q : Qp).
 
 (** ** Ghost state *)
+
+(** Algebra for the depth bounding *)
+Definition depthR := authR max_natR.
+Implicit Type d g : nat.
 
 (** ID for a borrower/lender *)
 Local Definition bor_id := positive.
 Local Definition lend_id := positive.
 Implicit Type (j : bor_id) (i : lend_id).
 
+(** Kind of a borrower *)
+Variant bor_kind :=
+| #[local] Clsd (* Closed *)
+| #[local] Open (q : Qp) (* Open with a fraction *)
+| #[local] Rebor (α : lft) (* Reborrowed *).
+Implicit Type b : bor_kind.
 (** State of a borrower *)
 Local Definition bor_st PROP : Type :=
-  PROP * option Qp (* Deposited fraction *).
+  PROP * bor_kind (* Deposited fraction *).
 (** State of the borrowers *)
 Local Definition bor_stm PROP : Type := gmap bor_id (bor_st PROP).
+
+(** Kind of a lender *)
+Variant lend_kind :=
+| #[local] Lend (* Lending *)
+| #[local] Dead (* Dead *).
+Implicit Type l : lend_kind.
 (** Core state of a lender *)
-Local Definition lend_cst PROP : Type :=
-  PROP * bool (* Whether lending or not *).
+Local Definition lend_cst PROP : Type := nat (* Depth *) * PROP * lend_kind.
 (** State of a lender *)
-Local Definition lend_st PROP : Type := lft * lend_cst PROP * bor_stm PROP.
+Local Definition lend_st PROP : Type :=
+  lft * lend_cst PROP * bor_stm PROP.
 (** State of the lenders *)
 Local Definition lend_stm PROP : Type := gmap lend_id (lend_st PROP).
-
-Implicit Type (α : lft) (b : option Qp) (l : bool).
 
 (** Algebra for a borrower *)
 Local Definition borR PROP := exclR (leibnizO (bor_st PROP)).
@@ -40,18 +55,31 @@ Local Definition lendR PROP := prodR
   (gmapR bor_id (borR PROP)).
 
 (** Algebra for the borrowing machinery *)
-Definition borrowR PROP := authR (gmapR lend_id (lendR PROP)).
+Definition borrowR_def PROP := authR (gmapR lend_id (lendR PROP)).
+Lemma borrowR_aux : seal borrowR_def. Proof. by eexists. Qed.
+Definition borrowR := borrowR_aux.(unseal).
+Lemma borrowR_unseal : borrowR = borrowR_def.
+Proof. exact: borrowR_aux.(seal_eq). Qed.
 
 (** Ghost state for the borrowing machinery *)
 Class borrowGS PROP Σ := BorrowGS {
+  borrowGS_lft :: lftG Σ;
+  borrowGS_depth :: inG Σ depthR;
   borrowGS_borrow :: inG Σ (borrowR PROP);
-  borrow_name : gname;
+  depth_name : gname; borrow_name : gname;
 }.
+Local Existing Instance borrowGS_depth.
 Local Existing Instance borrowGS_borrow.
+Local Instance inG_borrow_def `{!inG Σ (borrowR PROP)} :
+  inG Σ (borrowR_def PROP).
+Proof. rewrite -borrowR_unseal. apply _. Qed.
 Class borrowGpreS PROP Σ := BorrowGpreS {
+  borrowGpreS_lft :: lftG Σ;
+  borrowGpreS_depth :: inG Σ depthR;
   borrowGpreS_borrow :: inG Σ (borrowR PROP);
 }.
-Definition borrowΣ PROP : gFunctors := #[GFunctor (borrowR PROP)].
+Definition borrowΣ PROP : gFunctors :=
+  #[GFunctor lftR; GFunctor depthR; GFunctor (borrowR PROP)].
 #[export] Instance subG_borrow `{!subG (borrowΣ PROP) Σ} : borrowGpreS PROP Σ.
 Proof. solve_inG. Qed.
 
@@ -62,25 +90,71 @@ Section borrow.
   Implicit Type (P Q : PROP)
     (B : bor_st PROP) (L : lend_st PROP) (Lm : lend_stm PROP).
 
-  (** Borrower token *)
-  Local Definition bor_ijtok i j α B : iProp Σ :=
+  (** Witness of a depth *)
+  Local Definition depth d : iProp Σ := own depth_name (◯ (MaxNat d)).
+  (** Global bound of the depths *)
+  Local Definition gdepth g : iProp Σ := own depth_name (● (MaxNat g)).
+
+  (** Get [depth 0] *)
+  Local Lemma depth_0 : ⊢ |==> depth 0. Proof. apply own_unit. Qed.
+  (** Introduce a new depth *)
+  Local Lemma depth_alloc {g d} : gdepth g ==∗ ∃ g', gdepth g' ∗ depth d.
+  Proof.
+    iIntros "g". iMod (own_update with "g") as "[? $]"; [|by iExists _].
+    apply auth_update_alloc, local_update_unital_discrete=> ? _.
+    by rewrite left_id=> <-.
+  Qed.
+
+  (** Bounding by [gdepth] *)
+  Local Lemma depth_bound {g d} : gdepth g -∗ depth d -∗ ⌜d ≤ g⌝.
+  Proof.
+    iIntros "g d". iDestruct (own_valid_2 with "g d") as %v. iPureIntro.
+    by move: v=> /auth_both_valid_discrete [/max_nat_included ? _].
+  Qed.
+
+  (** General borrower token *)
+  Local Definition bor_itok i j α B : iProp Σ :=
     own borrow_name (◯ {[i := (to_agree α, ε, {[j := Excl B]})]}).
-  Definition bor_tok α P : iProp Σ := ∃ i j, bor_ijtok i j α (P, None).
-  Definition bor_otok `{!lftG Σ} α P q : iProp Σ :=
-    (q/2).[α] ∗ ∃ i j, bor_ijtok i j α (P, Some (q/2)%Qp).
+
+  (** Borrower token *)
+  Local Definition bor_tok_def α P : iProp Σ :=
+    [†α] ∨ ∃ i j,
+      bor_itok i j α (P, Clsd) ∨ ∃ β, [†β] ∗ bor_itok i j α (P, Rebor β).
+  Local Lemma bor_tok_aux : seal bor_tok_def. Proof. by eexists. Qed.
+  Definition bor_tok := bor_tok_aux.(unseal).
+  Local Lemma bor_tok_unseal : bor_tok = bor_tok_def.
+  Proof. exact: bor_tok_aux.(seal_eq). Qed.
+
+  (** Open borrower token *)
+  Local Definition bor_otok_def α P q : iProp Σ :=
+    (q/2).[α] ∗ ∃ i j, bor_itok i j α (P, Open (q/2)%Qp).
+  Local Lemma bor_otok_aux : seal bor_otok_def. Proof. by eexists. Qed.
+  Definition bor_otok := bor_otok_aux.(unseal).
+  Local Lemma bor_otok_unseal : bor_otok = bor_otok_def.
+  Proof. exact: bor_otok_aux.(seal_eq). Qed.
 
   (** Lender token *)
-  Local Definition lend_itok i α P : iProp Σ :=
-    own borrow_name (◯ {[i := (to_agree α, Excl' (P, true), ε)]}).
-  Definition lend_tok α P : iProp Σ := ∃ i, lend_itok i α P.
+  Local Definition lend_itok i α d P : iProp Σ :=
+    own borrow_name (◯ {[i := (to_agree α, Excl' (d, P, Lend), ε)]}).
+  Local Definition lend_dtok α d P : iProp Σ :=
+    depth d ∗ ∃ i, lend_itok i α d P.
+  Local Definition lend_tok_def α P : iProp Σ := ∃ d, lend_dtok α d P.
+  Local Lemma lend_tok_aux : seal lend_tok_def. Proof. by eexists. Qed.
+  Definition lend_tok := lend_tok_aux.(unseal).
+  Local Lemma lend_tok_unseal : lend_tok = lend_tok_def.
+  Proof. exact: lend_tok_aux.(seal_eq). Qed.
 
   (** Borrower and lender tokens are timeless *)
-  Fact bor_tok_timeless {α P} : Timeless (bor_tok α P).
-  Proof. apply _. Qed.
-  Fact bor_otok_timeless `{!lftG Σ} {α P q} : Timeless (bor_otok α P q).
-  Proof. apply _. Qed.
-  Fact lend_tok_timeless {α P} : Timeless (lend_tok α P).
-  Proof. apply _. Qed.
+  #[export] Instance bor_tok_timeless {α P} : Timeless (bor_tok α P).
+  Proof. rewrite bor_tok_unseal. apply _. Qed.
+  #[export] Instance bor_otok_timeless {α P q} : Timeless (bor_otok α P q).
+  Proof. rewrite bor_otok_unseal. apply _. Qed.
+  #[export] Instance lend_tok_timeless {α P} : Timeless (lend_tok α P).
+  Proof. rewrite lend_tok_unseal. apply _. Qed.
+
+  (** Fake a borrower from the dead lifetime token *)
+  Lemma bor_fake {α P} : [†α] ⊢ bor_tok α P.
+  Proof. rewrite bor_tok_unseal. iIntros. by iLeft. Qed.
 
   (** Token for [lend_stm] *)
   Local Definition lend_st_to_lendR L : lendR PROP :=
@@ -88,27 +162,66 @@ Section borrow.
   Local Definition lend_stm_tok Lm : iProp Σ :=
     own borrow_name (● (lend_st_to_lendR <$> Lm : gmapR _ _)).
 
-  (** Create [bor_ijtok] and [lend_itok] w.r.t. [lend_stm_tok] *)
-  Local Lemma lend_stm_create {Lm α P} :
+  (** Create [bor_itok] and [lend_itok] w.r.t. [lend_stm_tok] *)
+  Local Lemma lend_stm_create {Lm α P} d :
     lend_stm_tok Lm -∗ |==> ∃ i j,
-      lend_stm_tok (<[i := (α, (P, true), {[j := (P, None)]})]> Lm) ∗
-      bor_ijtok i j α (P, None) ∗ lend_itok i α P.
+      lend_stm_tok (<[i := (α, (d, P, Lend), {[j := (P, Clsd)]})]> Lm) ∗
+      bor_itok i j α (P, Clsd) ∗ lend_itok i α d P.
   Proof.
     iIntros "●". iExists (fresh (dom Lm)), 1%positive.
     iMod (own_update with "●") as "[$[$$]]"; [|done].
     rewrite -auth_frag_op singleton_op fmap_insert. apply auth_update_alloc.
-    have <-: lend_st_to_lendR (α, (P, true), {[1%positive := (P, None)]}) ≡
-      ((to_agree α, ε, {[1%positive := Excl (P, None)]}) : lendR _) ⋅
-        (to_agree α, Excl' (P, true), ε).
+    have <-: lend_st_to_lendR (α, (d, P, Lend), {[1%positive := (P, Clsd)]}) ≡
+      ((to_agree α, ε, {[1%positive := Excl (P, Clsd)]}) : lendR _) ⋅
+        (to_agree α, Excl' (d, P, Lend), ε).
     { split; [split|]=>/=; by [rewrite agree_idemp|]. }
     apply alloc_singleton_local_update.
     - rewrite lookup_fmap. apply fmap_None, not_elem_of_dom_1, is_fresh.
     - split; [split|]=>/=; by [|rewrite map_fmap_singleton singleton_valid].
   Qed.
 
-  (** Agreement between [lend_stm_tok] and [bor_ijtok] *)
+  (** Agreement between [lend_stm_tok] and [lend_itok] *)
+  Local Lemma lend_stm_lend_agree {Lm i α d P} :
+    lend_stm_tok Lm -∗ lend_itok i α d P -∗
+      ⌜∃ Bm, Lm !! i = Some (α, (d, P, Lend), Bm)⌝.
+  Proof.
+    iIntros "● l". iDestruct (own_valid_2 with "● l") as %v. iPureIntro.
+    move: v=> /auth_both_valid_discrete[/singleton_included_l[?[
+      /Some_equiv_eq[?[/lookup_fmap_Some[[[??]Bm][<-?]]<-]]
+      /Some_included_total/prod_included[/prod_included/=[
+        /to_agree_included/leibniz_equiv_iff?
+        /Excl_included/leibniz_equiv_iff?]_]]]_].
+    subst. by eexists _.
+  Qed.
+  (** Extend a lender w.r.t. [lend_stm_tok] *)
+  Local Lemma lend_stm_lend_extend {Lm i α d P Bm Q} :
+    Lm !! i = Some (α, (d, P, Lend), Bm) →
+    lend_stm_tok Lm -∗ lend_itok i α d P ==∗
+      lend_stm_tok (<[i := (α, (d, Q, Lend), Bm)]> Lm) ∗ lend_itok i α d Q.
+  Proof.
+    move=> ?. iIntros "● l". iMod (own_update_2 with "● l") as "[$$]"; [|done].
+    apply auth_update. rewrite fmap_insert. eapply singleton_local_update.
+    { rewrite lookup_fmap_Some. by eexists _. }
+    apply prod_local_update; [apply prod_local_update|]=>/=; [done| |done].
+    apply: option_local_update. by apply exclusive_local_update.
+  Qed.
+  (** Retrieve for a lender w.r.t. [lend_stm_tok] *)
+  Local Lemma lend_stm_lend_retrieve {Lm i α d P Bm} :
+    Lm !! i = Some (α, (d, P, Lend), Bm) →
+    lend_stm_tok Lm -∗ lend_itok i α d P ==∗
+      lend_stm_tok (<[i := (α, (d, P, Dead), Bm)]> Lm).
+  Proof.
+    move=> ?. iIntros "● l". iMod (own_update_2 with "● l") as "[$_]"; [|done].
+    apply auth_update. rewrite fmap_insert.
+    eapply (singleton_local_update _ _ _ _ _ (_,_,_)).
+    { rewrite lookup_fmap_Some. by eexists _. }
+    apply prod_local_update; [apply prod_local_update|]=>/=; [done| |done].
+    apply: option_local_update. by apply exclusive_local_update.
+  Qed.
+
+  (** Agreement between [lend_stm_tok] and [bor_itok] *)
   Local Lemma lend_stm_bor_agree {Lm i j α B} :
-    lend_stm_tok Lm -∗ bor_ijtok i j α B -∗
+    lend_stm_tok Lm -∗ bor_itok i j α B -∗
       ⌜∃ C Bm, Lm !! i = Some (α, C, Bm) ∧ Bm !! j = Some B⌝.
   Proof.
     iIntros "● B". iDestruct (own_valid_2 with "● B") as %v. iPureIntro.
@@ -124,8 +237,9 @@ Section borrow.
   (** Update the borrower state w.r.t. [lend_stm_tok] *)
   Local Lemma lend_stm_bor_stupd {Lm i j α C Bm B B'} :
     Lm !! i = Some (α, C, Bm) → Bm !! j = Some B →
-    lend_stm_tok Lm -∗ bor_ijtok i j α B ==∗
-      lend_stm_tok (<[i := (α, C, <[j := B']> Bm)]> Lm) ∗ bor_ijtok i j α B'.
+    lend_stm_tok Lm -∗ bor_itok i j α B ==∗
+      lend_stm_tok (<[i := (α, C, <[j := B']> Bm)]> Lm) ∗
+      bor_itok i j α B'.
   Proof.
     move=> ??. iIntros "● B". iMod (own_update_2 with "● B") as "[$$]"; [|done].
     apply auth_update. rewrite fmap_insert. eapply singleton_local_update.
@@ -137,7 +251,7 @@ Section borrow.
   (** Delete the borrower w.r.t. [lend_stm_tok] *)
   Local Lemma lend_stm_bor_delete {Lm i j α C Bm B} :
     Lm !! i = Some (α, C, Bm) → Bm !! j = Some B →
-    lend_stm_tok Lm -∗ bor_ijtok i j α B ==∗ ∃ Bm',
+    lend_stm_tok Lm -∗ bor_itok i j α B ==∗ ∃ Bm',
       lend_stm_tok (<[i := (α, C, Bm')]> Lm) ∗
       ⌜∀ Φ : _ → iProp Σ, ([∗ map] B ∈ Bm, Φ B) ⊣⊢ Φ B ∗ [∗ map] B ∈ Bm', Φ B⌝.
   Proof.
@@ -155,7 +269,7 @@ Section borrow.
   Local Lemma lend_stm_new_bor {Lm i α C Bm B} :
     Lm !! i = Some (α, C, Bm) →
     lend_stm_tok Lm ==∗ ∃ Bm', lend_stm_tok (<[i := (α, C, Bm')]> Lm) ∗
-      (∃ j, bor_ijtok i j α B) ∗
+      (∃ j, bor_itok i j α B) ∗
       ⌜∀ Φ : _ → iProp Σ, ([∗ map] B ∈ Bm', Φ B) ⊣⊢ Φ B ∗ [∗ map] B ∈ Bm, Φ B⌝.
   Proof.
     move=> Lmi. iIntros "●". iExists (<[fresh (dom Bm) := B]> Bm).
@@ -177,82 +291,50 @@ Section borrow.
   Local Lemma lend_stm_new_bors {Lm i α C Bm Bl} :
     Lm !! i = Some (α, C, Bm) →
     lend_stm_tok Lm ==∗ ∃ Bm', lend_stm_tok (<[i := (α, C, Bm')]> Lm) ∗
-      ([∗ list] B ∈ Bl, ∃ j, bor_ijtok i j α B) ∗
+      ([∗ list] B ∈ Bl, ∃ j, bor_itok i j α B) ∗
       ⌜∀ Φ : _ → iProp Σ,
         ([∗ map] B ∈ Bm', Φ B) ⊣⊢ ([∗ list] B ∈ Bl, Φ B) ∗ [∗ map] B ∈ Bm, Φ B⌝.
   Proof.
     move=> ?. elim: Bl=> /=[|B Bl IH].
-    { iIntros "●". iModIntro. iExists Bm. iSplit; [by rewrite insert_id|].
-      iSplit; [done|]. iPureIntro=> ?. by rewrite left_id. }
+    { iIntros "●". iModIntro. iExists Bm. rewrite insert_id; [|done].
+      iFrame "●". iSplit; [done|]. iPureIntro=> ?. by rewrite left_id. }
     iIntros "●". iMod (IH with "●") as (Bm') "[●[$ %eq]]".
     iMod (lend_stm_new_bor with "●") as (Bm'') "[●[$ %eq']]";
       [by rewrite lookup_insert|].
     rewrite insert_insert. iModIntro. iExists _. iSplit; [done|].
     iPureIntro=> ?. by rewrite -assoc -eq.
   Qed.
-
-  (** Agreement between [lend_stm_tok] and [lend_itok] *)
-  Local Lemma lend_stm_lend_agree {Lm i α P} :
-    lend_stm_tok Lm -∗ lend_itok i α P -∗
-      ⌜∃ Bm, Lm !! i = Some (α, (P, true), Bm)⌝.
-  Proof.
-    iIntros "● l". iDestruct (own_valid_2 with "● l") as %v. iPureIntro.
-    move: v=> /auth_both_valid_discrete[/singleton_included_l[?[
-      /Some_equiv_eq[?[/lookup_fmap_Some[[[??]Bm][<-?]]<-]]
-      /Some_included_total/prod_included[/prod_included/=[
-        /to_agree_included/leibniz_equiv_iff?
-        /Excl_included/leibniz_equiv_iff?]_]]]_].
-    subst. by eexists _.
-  Qed.
-  (** Extend a lender w.r.t. [lend_stm_tok] *)
-  Local Lemma lend_stm_lend_extend {Lm i α P Bm Q} :
-    Lm !! i = Some (α, (P, true), Bm) →
-    lend_stm_tok Lm -∗ lend_itok i α P ==∗
-      lend_stm_tok (<[i := (α, (Q, true), Bm)]> Lm) ∗ lend_itok i α Q.
-  Proof.
-    move=> ?. iIntros "● l". iMod (own_update_2 with "● l") as "[$$]"; [|done].
-    apply auth_update. rewrite fmap_insert. eapply singleton_local_update.
-    { rewrite lookup_fmap_Some. by eexists _. }
-    apply prod_local_update; [apply prod_local_update|]=>/=; [done| |done].
-    apply: option_local_update. by apply exclusive_local_update.
-  Qed.
-  (** Retrieve for a lender w.r.t. [lend_stm_tok] *)
-  Local Lemma lend_stm_lend_retrieve {Lm i α P Bm} :
-    Lm !! i = Some (α, (P, true), Bm) →
-    lend_stm_tok Lm -∗ lend_itok i α P ==∗
-      lend_stm_tok (<[i := (α, (P, false), Bm)]> Lm).
-  Proof.
-    move=> ?. iIntros "● l". iMod (own_update_2 with "● l") as "[$_]"; [|done].
-    apply auth_update. rewrite fmap_insert.
-    eapply (singleton_local_update _ _ _ _ _ (_,_,_)).
-    { rewrite lookup_fmap_Some. by eexists _. }
-    apply prod_local_update; [apply prod_local_update|]=>/=; [done| |done].
-    apply: option_local_update. by apply exclusive_local_update.
-  Qed.
 End borrow.
 
 (** ** World satisfactions *)
 
 Section borrow.
-  Context `{!lftG Σ, !borrowGS PROP Σ}.
+  Context `{!borrowGS PROP Σ}.
   Implicit Type (M : iProp Σ → iProp Σ) (intp : PROP → iProp Σ)
-    (P Q : PROP) (B : bor_st PROP) (Bm : bor_stm PROP).
+    (P Q : PROP) (B : bor_st PROP) (Bm : bor_stm PROP) (C : lend_cst PROP).
 
   (** World satisfaction for a borrower *)
-  Local Definition bor_wsat intp α B : iProp Σ :=
-    match B.2 with None => intp B.1 | Some q => q.[α] end.
+  Local Definition bor_wsat M intp α d B : iProp Σ :=
+    match B.2 with
+    | Clsd => M (intp B.1) | Open q => q.[α]
+    | Rebor β => lend_dtok (α ⊓ β) (S d) B.1
+    end.
 
   (** World satisfaction for a lender *)
-  Local Definition lend_wsat' M intp α P Bm : iProp Σ :=
-    ([∗ map] B ∈ Bm, bor_wsat intp α B) ∗
-    (([∗ map] B ∈ Bm, intp B.1) -∗ M (intp P)).
-  Local Definition lend_wsat M intp α P l Bm : iProp Σ :=
-    if l then lend_wsat' M intp α P Bm else [†α]%I.
+  Local Definition lend_wsat' M intp α d P Bm : iProp Σ :=
+    ([∗ map] B ∈ Bm, bor_wsat M intp α d B) ∗
+    ([†α] -∗ ([∗ map] B ∈ Bm, intp B.1) -∗ M (intp P)).
+  Local Definition lend_wsat M intp α C Bm : iProp Σ :=
+    match C.2 with
+    | Lend => lend_wsat' M intp α C.1.1 C.1.2 Bm | Dead => [†α]%I
+    end.
 
   (** World satisfaction for the borrowing machinery *)
+  Local Definition borrow_wsat' M intp g : iProp Σ :=
+    gdepth g ∗ ∃ Lm, lend_stm_tok Lm ∗
+      [∗ map] L ∈ Lm, lend_wsat M intp L.1.1 L.1.2 L.2.
   Local Definition borrow_wsat_def M intp : iProp Σ :=
-    ∃ Lm, lend_stm_tok Lm ∗
-      [∗ map] L ∈ Lm, lend_wsat M intp L.1.1 L.1.2.1 L.1.2.2 L.2.
+    ∃ g, borrow_wsat' M intp g.
   Local Definition borrow_wsat_aux : seal borrow_wsat_def.
   Proof. by eexists. Qed.
   Definition borrow_wsat := borrow_wsat_aux.(unseal).
@@ -260,17 +342,23 @@ Section borrow.
   Proof. exact: borrow_wsat_aux.(seal_eq). Qed.
 
   (** Non-expansiveness *)
-  #[export] Instance bor_wsat_ne :
-    Proper (pointwise_relation _ (⊣⊢) ==> (=) ==> (=) ==> (⊣⊢)) bor_wsat.
-  Proof. move=> ?? eq ??<-[?[?|]]?<-; by rewrite /bor_wsat/= ?eq. Qed.
-  #[export] Instance lend_wsat'_ne `{!GenUpd _ M} :
+  #[export] Instance bor_wsat_ne `{!GenUpd _ M} :
     Proper (pointwise_relation _ (⊣⊢) ==> (=) ==> (=) ==> (=) ==> (⊣⊢))
-      (lend_wsat' M).
-  Proof. move=> ?????<-??<-??<-. rewrite /lend_wsat'. repeat f_equiv. Qed.
-  #[export] Instance lend_wsat_ne `{!GenUpd _ M} :
+      (bor_wsat M).
+  Proof. move=> ?? eq ??<-??<-[?[|?|?]]?<-; by rewrite /bor_wsat/= ?eq. Qed.
+  #[export] Instance lend_wsat'_ne `{!GenUpd _ M} :
     Proper (pointwise_relation _ (⊣⊢) ==> (=) ==> (=) ==> (=) ==> (=) ==> (⊣⊢))
+      (lend_wsat' M).
+  Proof. move=> ?????<-??<-??<-??<-. rewrite /lend_wsat'. repeat f_equiv. Qed.
+  #[export] Instance lend_wsat_ne `{!GenUpd _ M} :
+    Proper (pointwise_relation _ (⊣⊢) ==> (=) ==> (=) ==> (=) ==> (⊣⊢))
       (lend_wsat M).
-  Proof. move=> ?????<-??<-[|]?<-??<-/=; by f_equiv. Qed.
+  Proof.
+    move=> ?????<-[[??][|]]?<-??<-; rewrite /lend_wsat/=; repeat f_equiv.
+  Qed.
+  #[export] Instance borrow_wsat'_ne `{!GenUpd _ M} :
+    Proper (pointwise_relation _ (⊣⊢) ==> (=) ==> (⊣⊢)) (borrow_wsat' M).
+  Proof. move=> ?????<-. rewrite /borrow_wsat'. repeat f_equiv. Qed.
   #[export] Instance borrow_wsat_ne `{!GenUpd _ M} :
     Proper (pointwise_relation _ (⊣⊢) ==> (⊣⊢)) (borrow_wsat M).
   Proof.
@@ -279,120 +367,235 @@ Section borrow.
 
   (** Create a borrower and a lender *)
   Lemma bor_lend_create `{!GenUpd _ M} {intp α P} :
-    intp P =[borrow_wsat M intp]=∗ bor_tok α P ∗ lend_tok α P.
+    M (intp P) =[borrow_wsat M intp]=∗ bor_tok α P ∗ lend_tok α P.
   Proof.
-    rewrite borrow_wsat_unseal. iIntros "P [%Lm[● Lm]]".
-    iMod (lend_stm_create with "●") as (??) "[● [b l]]"; [done..|]. iModIntro.
-    iSplitR "b l"; [|iSplitL "b"; by [iExists _, _|iExists _]]. iExists _.
-    iFrame "●". iApply (big_sepM_insert_2 with "[P] Lm")=>/=.
-    iSplitL; rewrite big_sepM_singleton; by [|iIntros].
-  Qed.
-
-  (** [lend_wsat] with a lifetime token *)
-  Local Lemma lend_wsat_tok {M intp q α P l Bm} :
-    q.[α] -∗ lend_wsat M intp α P l Bm -∗ ⌜l = true⌝.
-  Proof.
-    iIntros "α †". case: l; [done|]=>/=.
-    iDestruct (lft_tok_dead with "α †") as "[]".
-  Qed.
-  (** Update the borrower state *)
-  Local Lemma bor_stupd {M intp q i j α P b b'} :
-    q.[α] -∗ bor_ijtok i j α (P, b) -∗ bor_wsat intp α (P, b')
-      =[borrow_wsat M intp]=∗
-      q.[α] ∗ bor_ijtok i j α (P, b') ∗ bor_wsat intp α (P, b).
-  Proof.
-    rewrite borrow_wsat_unseal. iIntros "α b B' [%Lm[● Lm]]".
-    iDestruct (lend_stm_bor_agree with "● b") as %[[Q l][Bm[??]]].
-    iDestruct (big_sepM_insert_acc with "Lm") as "[L →Lm]"; [done|]=>/=.
-    iDestruct (lend_wsat_tok with "α L") as %->. iFrame "α".
-    iDestruct "L" as "[Bm →Q]".
-    iDestruct (big_sepM_insert_acc with "Bm") as "[$ →Bm]"; [done|].
-    iMod (lend_stm_bor_stupd with "● b") as "[● $]"; [done..|]. iModIntro.
-    iExists _. iFrame "●". iApply "→Lm"=>/=. iSplitR "→Q"; [by iApply "→Bm"|].
-    iStopProof. f_equiv=>/=. apply bi.equiv_entails_1_1.
-    by apply: big_sepM_insert_override.
-  Qed.
-  (** Open the borrower *)
-  Lemma bor_open {M intp q α P} :
-    bor_tok α P -∗ q.[α] =[borrow_wsat M intp]=∗ intp P ∗ bor_otok α P q.
-  Proof.
-    iIntros "[%i[%j b]] [α α']".
-    iMod (bor_stupd (b':=Some _) with "α b α'") as "[$[b $]]". by iExists _, _.
-  Qed.
-  (** Close the borrower *)
-  Lemma bor_close {M intp q α P} :
-    bor_otok α P q -∗ intp P =[borrow_wsat M intp]=∗ q.[α] ∗ bor_tok α P.
-  Proof.
-    iIntros "[α[%i[%j b]]] P".
-    iMod (bor_stupd (b':=None) with "α b P") as "[$[b $]]". by iExists _, _.
-  Qed.
-
-  (** Subdivide a borrower *)
-  Lemma bor_subdiv `{!GenUpd _ M} {intp q α P} Ql :
-    bor_otok α P q -∗ ([∗ list] Q ∈ Ql, intp Q) -∗
-    (([∗ list] Q ∈ Ql, intp Q) -∗ M (intp P)) =[borrow_wsat M intp]=∗
-      q.[α] ∗ [∗ list] Q ∈ Ql, bor_tok α Q.
-  Proof.
-    rewrite borrow_wsat_unseal. iIntros "[α[%i[%j b]]] Ql →P [%Lm[● Lm]]".
-    iDestruct (lend_stm_bor_agree with "● b") as %[[R l][Bm[??]]].
-    iDestruct (big_sepM_insert_acc with "Lm") as "[L →Lm]"; [done|]=>/=.
-    iDestruct (lend_wsat_tok with "α L") as %->=>/=. iFrame "α".
-    iMod (lend_stm_bor_delete with "● b") as (Bm') "[● %eq]"; [done..|].
-    iMod (lend_stm_new_bors (i:=i) (Bl:=(λ Q,(Q,None)) <$> Ql) with "●")
-      as (Bm'') "[● [bl %eq']]"; [by rewrite lookup_insert|]. iModIntro.
-    rewrite insert_insert big_sepL_fmap. iDestruct "L" as "[Bm →R]".
-    rewrite !eq. iDestruct "Bm" as "[$ Bm']". iSplitR "bl"; last first.
-    { iApply (big_sepL_mono with "bl")=> *. iIntros "[% ?]". by iExists _, _. }
-    iExists _. iFrame "●". iApply "→Lm"=>/=.
-    iSplitL "Ql Bm'"; rewrite eq' big_sepL_fmap /=; [by iFrame|].
-    iIntros "[Ql Bm']". iMod ("→P" with "Ql") as "P". iApply "→R". by iFrame.
+    rewrite borrow_wsat_unseal bor_tok_unseal lend_tok_unseal.
+    iIntros "P [%g[g[%Lm[● Lm]]]]". iMod depth_0 as "d".
+    iMod (lend_stm_create with "●") as (??) "[●[b l]]"; [done..|]. iModIntro.
+    iSplitR "b l d"; last first.
+    { iSplitL "b"; [|iExists _; iFrame "d"; by iExists _].
+      iRight. iExists _, _. by iLeft. }
+    iExists _. iFrame "g". iExists _. iFrame "●".
+    iApply (big_sepM_insert_2 with "[P] Lm")=>/=.
+    iSplitL; rewrite big_sepM_singleton /=; by [iLeft|iIntros].
   Qed.
 
   (** Extend the lender token *)
   Lemma lend_extend `{!GenUpd _ M} {intp α P Q} :
-    lend_tok α P -∗ (intp P -∗ M (intp Q)) =[borrow_wsat M intp]=∗ lend_tok α Q.
+    lend_tok α P -∗ ([†α] -∗ intp P -∗ M (intp Q)) =[borrow_wsat M intp]=∗
+      lend_tok α Q.
   Proof.
-    rewrite borrow_wsat_unseal. iIntros "[%i l] PQ [%Lm[● Lm]]".
+    rewrite lend_tok_unseal borrow_wsat_unseal.
+    iIntros "[%d[d[%i l]]] PQ [%g[g[%Lm[● Lm]]]]".
     iDestruct (lend_stm_lend_agree with "● l") as %[Bm ?].
     iDestruct (big_sepM_insert_acc with "Lm") as "[L →Lm]"; [done|]=>/=.
     iMod (lend_stm_lend_extend with "● l") as "[● l]"; [done|]. iModIntro.
-    iSplitR "l"; [|by iExists _]. iExists _. iFrame "●". iApply "→Lm"=>/=.
-    iDestruct "L" as "[$ →P]". iIntros "Bm". iMod ("→P" with "Bm") as "P".
-    by iApply "PQ".
+    iSplitR "d l"; [|iExists _; iFrame "d"; by iExists _]. iExists _.
+    iFrame "g". iExists _. iFrame "●". iApply "→Lm"=>/=.
+    iDestruct "L" as "[$ →P]"=>/=. iIntros "#† Bm".
+    iMod ("→P" with "† Bm") as "P". by iApply "PQ".
   Qed.
 
   (** [bor_wsat] with the dead lifetime token *)
-  Local Lemma bor_wsat_dead {intp α B} : [†α] -∗ bor_wsat intp α B -∗ intp B.1.
+  Local Lemma bor_wsat_dead {M intp α d B} :
+    [†α] -∗ bor_wsat M intp α d B -∗
+      M (intp B.1) ∨ ∃ β, lend_dtok (α ⊓ β) (S d) B.1.
   Proof.
-    case B=> [P[q|]]=>/=; [|by iIntros]. iIntros "† q".
-    iDestruct (lft_tok_dead with "q †") as "[]".
+    case B=> /=[P[|q|?]]; [iIntros; by iLeft| |iIntros; iRight; by iExists _].
+    iIntros "† q". iDestruct (lft_tok_dead with "q †") as "[]".
+  Qed.
+  Local Lemma bor_wsat_list_dead `{!GenUpd _ M} {intp α d Bl} {p q : iProp _} :
+    [†α] -∗ ([∗ list] B ∈ Bl, bor_wsat M intp α d B) -∗
+    (([∗ list] B ∈ Bl, intp B.1) -∗ p -∗ M q) -∗ ∃ Ql,
+      ([∗ list] Q ∈ Ql, ∃ β, lend_dtok (α ⊓ β) (S d) Q) ∗
+      (([∗ list] Q ∈ Ql, intp Q) -∗ p -∗ M q).
+  Proof.
+    move: p. elim: Bl=>/= [|[Q b] Bl IH p].
+    { iIntros. iExists []. by iSplit. } iIntros "#† [B Bl] →q".
+    iDestruct (IH (_∗_)%I with "† Bl [→q]") as (Ql) "[Ql →q]".
+    { iIntros "Bl [Q p]". by iApply ("→q" with "[$Bl Q] p"). }
+    iDestruct (bor_wsat_dead with "† B") as "[Q|l]";
+      [iExists Ql|iExists (Q :: Ql)]=>/=; iFrame "Ql"; [|iFrame "l"];
+      [iIntros "Ql p"; iMod "Q"|iIntros "[Q Ql] p"];
+      iApply ("→q" with "Ql [$Q $p]").
   Qed.
   (** [lend_wsat'] with the dead lifetime token *)
-  Local Lemma lend_wsat'_dead {M intp α P Bm} :
-    [†α] -∗ lend_wsat' M intp α P Bm -∗ M (intp P).
+  Local Lemma big_sepM_map_to_list_snd (Φ : _ → iProp Σ) Bm :
+    ([∗ map] B ∈ Bm, Φ B) ⊣⊢ [∗ list] B ∈ (map_to_list Bm).*2, Φ B.
+  Proof. by rewrite big_sepM_map_to_list big_sepL_fmap. Qed.
+  Local Lemma lend_wsat'_dead `{!GenUpd _ M} {intp α d P Bm} :
+    [†α] -∗ lend_wsat' M intp α d P Bm -∗ ∃ Ql,
+      ([∗ list] Q ∈ Ql, ∃ β, lend_dtok (α ⊓ β) (S d) Q) ∗
+      (([∗ list] Q ∈ Ql, intp Q) -∗ M (intp P)).
   Proof.
-    iIntros "#† [Bm →P]". iApply "→P". iApply (big_sepM_impl with "Bm").
-    iIntros "!>" (?? _). by iApply bor_wsat_dead.
+    iIntros "#† [Bl →P]". iDestruct ("→P" with "†") as "→P".
+    rewrite !big_sepM_map_to_list_snd. move: (map_to_list Bm).*2=> Bl.
+    iDestruct (bor_wsat_list_dead (p:=True) with "† Bl [→P]") as (Ql) "[Ql →P]".
+    { iIntros "Bl _".  by iApply ("→P" with "Bl"). }
+    iExists _. iFrame "Ql". iIntros "Ql". by iApply ("→P" with "Ql").
   Qed.
-  (** Retrieve from the lender token *)
-  Lemma lend_retrieve {M intp α P} :
-    [†α] -∗ lend_tok α P =[borrow_wsat M intp]=∗ M (intp P).
+  (** Retrieve from the lender token with remaining lender tokens *)
+  Local Lemma lend_pre_retrieve `{!GenUpd _ M} {intp g α d P} :
+    [†α] -∗ lend_dtok α d P =[borrow_wsat' M intp g]=∗ ∃ Ql,
+      ([∗ list] Q ∈ Ql, ∃ β, lend_dtok (α ⊓ β) (S d) Q) ∗
+      (([∗ list] Q ∈ Ql, intp Q) -∗ M (intp P)).
   Proof.
-    rewrite borrow_wsat_unseal. iIntros "#† [%i l] [%Lm[● Lm]]".
+    iIntros "#† [d[%i l]] [$[%Lm[● Lm]]]".
     iDestruct (lend_stm_lend_agree with "● l") as %[Bm ?].
     iDestruct (big_sepM_insert_acc with "Lm") as "[L →Lm]"; [done|]=>/=.
     iDestruct (lend_wsat'_dead with "† L") as "$". iExists _.
     iMod (lend_stm_lend_retrieve with "● l") as "$"; by [|iApply "→Lm"].
   Qed.
+  (** Retrieve from the lender token,
+    by induction on (the maximum depth minus) the depth *)
+  Local Lemma lend_retrieve' `{!GenUpd _ M} {intp k α d P} :
+    [†α] -∗ lend_dtok α d P =[borrow_wsat' M intp (d + k)]=∗ M (intp P).
+  Proof.
+    move: α d P. elim: k=> [|k IH] α d P; iIntros "#† l";
+      iMod (lend_pre_retrieve with "† l") as (Ql) "[Ql →P]".
+    { case: Ql=> /=[|??]. { by iDestruct ("→P" with "[//]") as "$". }
+      iDestruct "Ql" as "[[%[Sd _]]_]". iIntros "[g _]".
+      iDestruct (depth_bound with "g Sd") as %?. lia. }
+    have ->: d + S k = S d + k by lia. iInduction Ql as [|Q Ql] "IH"=>/=.
+    { by iDestruct ("→P" with "[//]") as "$". }
+    iDestruct "Ql" as "[[%β l] Ql]".
+    iMod (IH with "[†] l") as "Q"; [by rewrite lft_dead_meet_l|].
+    iApply ("IH" with "Ql"). iIntros "Ql". iMod "Q". iApply "→P". iFrame.
+  Qed.
+  Lemma lend_retrieve `{!GenUpd _ M} {intp α P} :
+    [†α] -∗ lend_tok α P =[borrow_wsat M intp]=∗ M (intp P).
+  Proof.
+    rewrite lend_tok_unseal borrow_wsat_unseal. iIntros "† [%d[d l]] [%g[g W]]".
+    iDestruct (depth_bound with "g d") as %le. move: le=> /Nat.le_sum[?->].
+    iMod (lend_retrieve' with "† [$d $l] [$g $W]") as "[W $]". by iExists _.
+  Qed.
+
+  (** [lend_wsat] with a lifetime token *)
+  Local Lemma lend_wsat_tok {M intp q α d Q l Bm} :
+    q.[α] -∗ lend_wsat M intp α (d, Q, l) Bm -∗ ⌜l = Lend⌝.
+  Proof.
+    iIntros "α †". case: l; by [|iDestruct (lft_tok_dead with "α †") as "[]"].
+  Qed.
+  (** Update the borrower state *)
+  Local Lemma bor_stupd {M intp q i j α P b b'} :
+    q.[α] -∗ bor_itok i j α (P, b) -∗ (∀ d, bor_wsat M intp α d (P, b'))
+      =[borrow_wsat M intp]=∗
+      q.[α] ∗ bor_itok i j α (P, b') ∗ ∃ d, bor_wsat M intp α d (P, b).
+  Proof.
+    rewrite borrow_wsat_unseal. iIntros "α b B' [%g[g[%Lm[● Lm]]]]".
+    iDestruct (lend_stm_bor_agree with "● b") as %[[[d Q]l][Bm[??]]].
+    iDestruct (big_sepM_insert_acc with "Lm") as "[L →Lm]"; [done|]=>/=.
+    iDestruct (lend_wsat_tok with "α L") as %->. iFrame "α".
+    iDestruct "L" as "[Bm →Q]".
+    iDestruct (big_sepM_insert_acc with "Bm") as "[B →Bm]"; [done|].
+    iMod (lend_stm_bor_stupd with "● b") as "[● $]"; [done..|]. iModIntro.
+    iSplitR "B"; [|by iExists _]. iExists _. iFrame "g". iExists _. iFrame "●".
+    iApply "→Lm". iSplitR "→Q"=>/=; [by iApply "→Bm"|]. iStopProof.
+    do 2 f_equiv. apply bi.equiv_entails_1_1.
+    by apply: big_sepM_insert_override.
+  Qed.
+  (** Open the borrower *)
+  Lemma bor_open `{!GenUpd _ M} {intp q α P} :
+    bor_tok α P -∗ q.[α] =[borrow_wsat M intp]=∗ M (intp P) ∗ bor_otok α P q.
+  Proof.
+    rewrite bor_tok_unseal bor_otok_unseal.
+    iIntros "[†|[%i[%j[b|[%β[#† b]]]]]] [α α']";
+      [iDestruct (lft_tok_dead with "α †") as "[]"| |];
+      iMod (bor_stupd (b':=Open _) with "α b [α']") as "[$[b[%d b']]]";
+      [by iIntros| |by iIntros|]; iSplitL "b'";
+      [done|by iExists _, _| |by iExists _, _].
+    rewrite lft_dead_meet_r. iApply (lend_retrieve with "† [b']").
+    rewrite lend_tok_unseal. by iExists _.
+  Qed.
+  (** Close the borrower *)
+  Lemma bor_close {M intp q α P} :
+    bor_otok α P q -∗ M (intp P) =[borrow_wsat M intp]=∗ q.[α] ∗ bor_tok α P.
+  Proof.
+    rewrite bor_otok_unseal bor_tok_unseal. iIntros "[α[%i[%j b]]] P".
+    iMod (bor_stupd (b':=Clsd) with "α b [P]") as "[$[b[% $]]]"; [by iIntros|].
+    iModIntro. iRight. iExists _, _. by iLeft.
+  Qed.
+
+  (** Reborrow a borrower *)
+  Local Lemma turn_rebor `{!GenUpd _ M} {intp α β R r} :
+    bor_tok β R -∗ r.[β] =[borrow_wsat M intp]=∗
+      bor_tok (α ⊓ β) R ∗ ([†α] -∗ bor_tok β R) ∗ r.[β].
+  Proof.
+    iIntros "b β". iMod (bor_open with "b β") as "[R o]".
+    rewrite bor_otok_unseal. iDestruct "o" as "[β[%i[%j o]]]".
+    rewrite borrow_wsat_unseal. iIntros "[%g[g[%Lm[● Lm]]]]".
+    iDestruct (lend_stm_bor_agree with "● o") as %[[[d Q]l][Bm[??]]].
+    iDestruct (big_sepM_insert_acc with "Lm") as "[L →Lm]"; [done|]=>/=.
+    iDestruct (lend_wsat_tok with "β L") as %->. iFrame "β".
+    iMod (lend_stm_bor_stupd (B':=(_,Rebor α)) with "● o") as "[● r]";
+      [done..|].
+    iMod (lend_stm_create with "●") as (i' j') "[● [b l]]"; [done..|].
+    iMod (depth_alloc with "g") as (g') "[g d]".
+    iModIntro. iDestruct "L" as "[Bm →Q]"=>/=.
+    iDestruct (big_sepM_insert_acc with "Bm") as "[B →Bm]"; [done|]. iFrame "B".
+    iSplitR "b r"; last first.
+    { rewrite bor_tok_unseal. iSplitL "b"; [|iIntros "†"]; iRight; iExists _, _;
+        by [iLeft|iRight; iExists _; iFrame]. }
+    iExists _. iFrame "g". iExists _. iFrame "●".
+    iApply (big_sepM_insert_2 with "[R]")=>/=.
+    { iSplitL; rewrite big_sepM_singleton /=; by [|iIntros]. }
+    iApply "→Lm". iSplitR "→Q"=>/=.
+    { iApply "→Bm". iFrame "d". rewrite comm. by iExists _. }
+    iStopProof. do 2 f_equiv. apply bi.equiv_entails_1_1.
+    by apply: big_sepM_insert_override.
+  Qed.
+  Local Lemma turn_rebors `{!GenUpd _ M} {intp α Rβrl} :
+    ([∗ list] Rβr ∈ Rβrl, bor_tok Rβr.1.2 Rβr.1.1 ∗ Rβr.2.[Rβr.1.2])
+      =[borrow_wsat M intp]=∗
+      ([∗ list] Rβr ∈ Rβrl, bor_tok (α ⊓ Rβr.1.2) Rβr.1.1 ∗ Rβr.2.[Rβr.1.2]) ∗
+      ([†α] -∗ [∗ list] Rβr ∈ Rβrl, bor_tok Rβr.1.2 Rβr.1.1).
+  Proof.
+    elim: Rβrl=> [|[[R β]r]RBql IH]/=. { iIntros "_!>". by iSplit; [|iIntros]. }
+    iIntros "[[b β] Rβrl]". iMod (IH with "Rβrl") as "[$ →bl]".
+    iMod (turn_rebor with "b β") as "[$[→b $]]". iIntros "!> #†".
+    iDestruct ("→b" with "†") as "$". by iApply "→bl".
+  Qed.
+  (** Subdivide a borrower *)
+  Lemma bor_subdiv `{!GenUpd _ M} {intp q α P} Ql Rβrl :
+    bor_otok α P q -∗ ([∗ list] Q ∈ Ql, intp Q) -∗
+    ([∗ list] Rβr ∈ Rβrl, bor_tok Rβr.1.2 Rβr.1.1 ∗ Rβr.2.[Rβr.1.2]) -∗
+    (([∗ list] Q ∈ Ql, intp Q) -∗
+      ([∗ list] Rβr ∈ Rβrl, bor_tok Rβr.1.2 Rβr.1.1) -∗ M (intp P))
+      =[borrow_wsat M intp]=∗
+      q.[α] ∗ ([∗ list] Q ∈ Ql, bor_tok α Q) ∗
+      [∗ list] Rβr ∈ Rβrl, bor_tok (α ⊓ Rβr.1.2) Rβr.1.1 ∗ Rβr.2.[Rβr.1.2].
+  Proof.
+    rewrite bor_otok_unseal. iIntros "[α[%i[%j b]]] Ql Rβrl →P".
+    iMod (turn_rebors with "Rβrl") as "[$ Rβrl]". rewrite borrow_wsat_unseal.
+    iIntros "[%g[g[%Lm[● Lm]]]]".
+    iDestruct (lend_stm_bor_agree with "● b") as %[[[d R]l][Bm[??]]].
+    iDestruct (big_sepM_insert_acc with "Lm") as "[L →Lm]"; [done|]=>/=.
+    iDestruct (lend_wsat_tok with "α L") as %->=>/=. iFrame "α".
+    iMod (lend_stm_bor_delete with "● b") as (Bm') "[● %eq]"; [done..|].
+    iMod (lend_stm_new_bors (i:=i) (Bl:=(λ Q,(Q,Clsd)) <$> Ql) with "●") as
+      (Bm'') "[● [bl %eq']]"; [by rewrite lookup_insert|]. iModIntro.
+    rewrite insert_insert big_sepL_fmap. iDestruct "L" as "[Bm →R]".
+    rewrite !eq. iDestruct "Bm" as "[$ Bm']". iSplitR "bl"; last first.
+    { iApply (big_sepL_mono with "bl")=> *. iIntros "[% ?]".
+      rewrite bor_tok_unseal. iRight. iExists _, _. by iLeft. }
+    iExists _. iFrame "g". iExists _. iFrame "●". iApply "→Lm"=>/=.
+    iSplitL "Bm' Ql"; rewrite !eq' !big_sepL_fmap /=.
+    { iFrame "Bm'". iStopProof. do 3 f_equiv. rewrite /bor_wsat/=. by iIntros. }
+    iIntros "#† [Ql Bm]".
+    iMod ("→P" with "Ql [Rβrl]") as "P"; [by iApply "Rβrl"|].
+    iApply ("→R" with "†"). iFrame.
+  Qed.
 End borrow.
 
 (** Allocate [borrow_wsat] *)
-Lemma borrow_wsat_alloc `{!lftG Σ, !borrowGpreS PROP Σ} :
+Lemma borrow_wsat_alloc `{!borrowGpreS PROP Σ} :
   ⊢ |==> ∃ _ : borrowGS PROP Σ, ∀ M intp, borrow_wsat M intp.
 Proof.
-  iMod (own_alloc (● ∅)) as (γ) "●"; [by apply auth_auth_valid|]. iModIntro.
-  iExists (BorrowGS _ _ _ γ). iIntros (M intp). rewrite borrow_wsat_unseal.
-  iExists ∅. by iFrame "●".
+  iMod (own_alloc (● (MaxNat 0))) as (γ) "g"; [by apply auth_auth_valid|].
+  iMod (own_alloc (● (∅ : gmapR _ _))) as (γ') "●";
+    [by apply auth_auth_valid|]. iModIntro.
+  iExists (BorrowGS _ _ _ _ _ γ γ'). iIntros (M intp).
+  rewrite borrow_wsat_unseal. iExists _. iFrame "g". iExists ∅. by iFrame.
 Qed.
 
 (** ** Fractured borrowing *)
@@ -418,18 +621,19 @@ Section borrow.
   Proof. iIntros "b". iApply (inv_alloc borN _). by iExists _. Qed.
 
   (** Open [frbor_tok] *)
-  Lemma frbor_open `{!lftG Σ, !GenUpd _ M} {intp Φ α q E} :
+  Lemma frbor_open `{!GenUpd _ M} {intp Φ α q W E} :
+    ElimModalS M (λ P, |=[W]{E ∖ ↑borN}=> P)%I →
+    ElimModalS
+      (λ P, |=[borrow_wsat M intp]=> P)%I (λ P, |=[W]{E ∖ ↑borN}=> P)%I →
     ↑borN ⊆ E → Fractional (intp ∘ Φ) →
-    frbor_tok α Φ -∗ q.[α] =[borrow_wsat M intp]{E}=∗ ∃ r,
-      intp (Φ r) ∗ bor_otok α (Φ r) q.
+    frbor_tok α Φ -∗ q.[α] =[W]{E}=∗ ∃ r, M (intp (Φ r)) ∗ bor_otok α (Φ r) q.
   Proof.
-    move=> ??. iIntros "#i α". iInv "i" as ">[%r b]".
-    iMod (bor_open with "b α") as "[Φ b]".
+    move=> ????. iIntros "#i α". iInv "i" as ">[%r b]".
+    iMod (bor_open with "b α") as "[>Φ b]".
     have eq: intp (Φ r) ⊣⊢ intp (Φ (r/2)%Qp) ∗ intp (Φ (r/2)%Qp).
     { by erewrite fractional_half; [|apply: fractional_as_fractional]. }
-    iMod (bor_subdiv [_;_] with "b [Φ] []") as "[α[b[b' _]]]";
-      rewrite ?eq; [by iDestruct "Φ" as "[$$]"|by iIntros "[$[$_]]"|].
-    iModIntro. iSplitL "b'"; [by iExists _|].
-    iMod (bor_open with "b α") as "?". by iExists _.
+    iMod (bor_subdiv [_;_] [] with "b [Φ] [] []") as "[α[[b[b' _]]_]]"=>/=;
+      rewrite ?eq; [by iDestruct "Φ" as "[$$]"|done|by iIntros "[$[$_]]"|].
+    iMod (bor_open with "b α") as "?". iModIntro. iSplitL "b'"; by iExists _.
   Qed.
 End borrow.
